coq: set theory

coq/set/Core/Semantics.v
@@ -5,78 +5,83 @@ Require Import Core.Elem.
 Require Import Core.Syntax.
 Require Import Core.Environment.
 
-Fixpoint toProp (e:Env) (p:Formula) : Prop :=
+Fixpoint eval (e:Env) (p:Formula) : Prop :=
     match p with
     | Bot           => False
     | Elem n m      => (e n) :: (e m)
-    | Imp p1 p2     => toProp e p1 -> toProp e p2
-    | All n p1      => forall (x:set), toProp (bind e n x) p1
+    | Imp p1 p2     => eval e p1 -> eval e p2
+    | All n p1      => forall (x:set), eval (bind e n x) p1
     end.
 
+
 (* Evaluation in empty environment. Should only be used for closed formulas.    *)
-Definition eval (p:Formula) : Prop := toProp env0 p.
+Definition eval0 (p:Formula) : Prop := eval env0 p.
 
 (* Evaluation with single binding 'n := x'. Should be used when only 'n' free.  *)
-Definition eval1 (n:nat) (x:set) (p:Formula) : Prop := toProp (env1 n x) p.
+Definition eval1 (n:nat) (x:set) (p:Formula) : Prop := eval (env1 n x) p.
 
 (* Evaluation with two bindings 'n := x' and 'm := y' (in that order).          *)
-Definition eval2 (n m:nat)(x y:set)(p:Formula):Prop := toProp (env2 n m x y) p.
+Definition eval2 (n m:nat)(x y:set)(p:Formula):Prop := eval (env2 n m x y) p.
 
-Lemma evalBot : eval Bot <-> False.
-Proof. firstorder. Qed.
 
-Lemma evalElem2 : forall (n m:nat) (x y:set), n <> m ->
-    eval2 n m x y (Elem n m) <-> x :: y. 
+Lemma evalBot : forall (e:Env), eval e Bot <-> False.
+Proof. intros e. unfold eval. split; intros H; assumption. Qed.
+
+Lemma evalElem : forall (e:Env) (n m:nat), 
+    eval e (Elem n m) <-> (e n) :: (e m).
+Proof. intros e n m. unfold eval. split; intros H; assumption. Qed.
+
+Lemma evalImp : forall (e:Env) (p q:Formula),
+    eval e (Imp p q) <-> (eval e p -> eval e q).
 Proof.
-    intros n m x y H. unfold eval2. unfold toProp.
-    rewrite env2_y. rewrite env2_x.
-    - tauto.
-    - assumption.
+    intros e p q. unfold eval. fold (eval e p). fold (eval e q).
+    split; intros H; assumption.
 Qed.
 
-
-(*
-
-Lemma evalImp : forall (p q:Formula),
-    eval (Imp p q) <-> eval p -> eval q.
-Proof. firstorder. Qed.
-
-Lemma evalAll : forall (p:Formula) (n:nat),
-    eval (All n p) <-> forall (x:set), eval1 n x p.
-Proof. firstorder. Qed.
-
-Lemma evalNot : forall (p:Formula), 
-    eval (Not p) <-> ~ eval p.
-Proof. firstorder. Qed.
-
-Lemma evalOr : LEM -> forall (p q:Formula), 
-    eval(Or p q) <-> eval p \/ eval q.
+Lemma evalAll : forall (e:Env) (p:Formula) (n:nat),
+    eval e (All n p) <-> forall (x:set), eval (bind e n x) p.
 Proof.
-    intros L p q. unfold Or, eval. simpl. 
+    intros e p n. unfold eval. split; intros H; assumption.
+Qed.
+
+Lemma evalNot : forall (e:Env) (p:Formula), 
+    eval e (Not p) <-> ~ eval e p.
+Proof. 
+    intros e p. unfold Not, eval. fold (eval e p).
+    split; intros H; assumption.
+Qed.
+
+Lemma evalOr : LEM -> forall (e:Env) (p q:Formula), 
+    eval e (Or p q) <-> eval e p \/ eval e q.
+Proof.
+    intros L e p q. unfold Or, eval. simpl. 
     apply LEMOr. assumption.
 Qed.
 
-Lemma evalAnd : LEM -> forall (p q:Formula),
-    eval(And p q) <-> eval p /\ eval q.
+Lemma evalAnd : LEM -> forall (e:Env) (p q:Formula),
+    eval e (And p q) <-> eval e p /\ eval e q.
 Proof.
-    intros L p q. unfold And, eval. simpl. 
+    intros L e p q. unfold And, eval. simpl. 
     apply LEMAnd. assumption.
 Qed.
 
-Lemma evalExi : LEM -> forall (p:Formula) (n:nat),
-    eval (Exi n p) <-> exists (x:set), eval1 n x p.
+Lemma evalExi : LEM -> forall (e:Env) (p:Formula) (n:nat),
+    eval e (Exi n p) <-> exists (x:set), eval (bind e n x) p.
 Proof.
-    intros L p n. unfold Exi, eval, eval1, env1. simpl. 
+    intros L e p n. unfold Exi, eval, bind. simpl. 
     apply LEMExist. assumption.
 Qed.
 
+
 Definition P1 : Formula := All 0 (All 1 (Elem 0 1)).
 
-Lemma evalP1 : eval P1 <-> forall (x y:set), x :: y.
+Lemma evalP1 : forall (e:Env), eval e P1 <-> forall (x y:set), x :: y.
 Proof.
-    firstorder.
+    intros e. unfold P1, eval, bind. simpl. 
+    split; intros H; assumption.
 Qed.
 
+(*
 (* There exists an empty set                                                    *)
 Definition P2 : Formula := Exi 0 (All 1 (Not (Elem 1 0))).
 
@@ -84,8 +89,4 @@ Lemma evalP2 : LEM -> eval P2 <-> exists (x:set), forall (z:set), ~ (z :: x).
 Proof.
     intros L. apply evalExi. assumption.
 Qed.
-
 *)
-
-
-
